systems/IdentifierSpaces.v
@@ -1,0 +1,203 @@
+Require Bool.Bvector.
+Require Vectors.VectorEq.
+Require Import ZArith.
+Require Zdigits.
+Require Omega.
+Require Import List.
+Import List.ListNotations.
+Require String.
+Require Import StructTact.StructTactics.
+
+(* This file defines and provides some lemmas about identifier spaces. An
+ * identifier is the hash of a name, which is a string. The space of all
+ * identifiers produced by a given hash function is cyclically ordered.
+ * However, this cyclic ordering can be unrolled into a linear one. All
+ * operations defined on identifiers are lifted to pointers, which are pairs of
+ * a name and the hash of that name, i.e., its identifier. *)
+
+Section IdentifierSpaces.
+  Variable N : nat.
+  Definition id := Bvector.Bvector N.
+  Definition name := String.string.
+  Variable hash : name -> id.
+  Record pointer := mkPointer { ptrId : id;
+                                ptrAddr : name }.
+
+  Definition make_pointer (n : name) : pointer :=
+    {| ptrId := hash n;
+       ptrAddr := n |}.
+
+  Definition id_of : pointer -> id :=
+    ptrId.
+
+  Definition addr_of : pointer -> name :=
+    ptrAddr.
+
+  Lemma make_pointer_correct_addr :
+    forall p a,
+      p = make_pointer a ->
+      addr_of p = a.
+  Proof.
+    intros.
+    now find_rewrite.
+  Qed.
+
+  Lemma make_pointer_correct_id :
+    forall p a,
+      p = make_pointer a ->
+      id_of p = hash a.
+  Proof.
+    intros.
+    now find_rewrite.
+  Qed.
+
+  Definition id_eq_dec : forall a b : id, {a = b} + {a <> b} :=
+    VectorEq.eq_dec _ Bool.eqb Bool.eqb_true_iff _.
+
+  Definition pointer_eq_dec : forall x y : pointer,
+      {x = y} + {x <> y}.
+  Proof.
+    intros.
+    repeat decide equality;
+      apply id_eq_dec.
+  Defined.
+
+  Definition z_of_id : id -> Z :=
+    Zdigits.binary_value N.
+
+  Definition id_of_z : Z -> id :=
+    Zdigits.Z_to_binary N.
+
+  Lemma z_of_id_inv :
+    forall x,
+      id_of_z (z_of_id x) = x.
+  Proof.
+    unfold id_of_z, z_of_id.
+    apply Zdigits.binary_to_Z_to_binary.
+  Qed.
+
+  Definition bv_ltb (x y : id) : bool :=
+    Z.ltb (z_of_id x) (z_of_id y).
+
+  (* true iff x in (a, b) on some sufficiently large "circle" *)
+  Definition between_bool (a x b : id) : bool :=
+    match bv_ltb a b, bv_ltb a x, bv_ltb x b with
+    | true, true, true => true
+    | false, true, _ => true
+    | false, _, true => true
+    | _, _, _ => false
+    end.
+
+  Lemma bv_ltb_antisymmetric :
+    forall x y,
+      bv_ltb x y = true ->
+      ~ bv_ltb y x = true.
+  Proof.
+    unfold bv_ltb in *.
+    intros.
+    rewrite Z.ltb_lt in *.
+    omega.
+  Qed.
+
+  Definition ptr_between_bool (a x b : pointer) : bool :=
+    between_bool (ptrId a) (ptrId x) (ptrId b).
+
+  (* this is a total linear less-than-or-equal relation, see proofs below *)
+  Definition unroll_between (h : id) (x y : id) : bool :=
+    if id_eq_dec h x
+    then true
+    else if id_eq_dec h y
+         then false
+         else if id_eq_dec x y
+              then true
+              else between_bool h x y.
+
+  Lemma unrolling_makes_h_least :
+    forall h x,
+      unroll_between h h x = true.
+  Proof.
+    unfold unroll_between.
+    intros.
+    break_if; auto.
+  Qed.
+
+  Lemma between_bool_yz_antisymmetric :
+    forall x y z,
+      between_bool x y z = true ->
+      ~ between_bool x z y = true.
+  Proof.
+    unfold between_bool.
+    intros.
+    repeat break_if; try find_eapply_lem_hyp bv_ltb_antisymmetric;
+      congruence.
+  Qed.
+
+  Lemma unrolling_antisymmetric :
+    forall h x y,
+      unroll_between h x y = true ->
+      unroll_between h y x = true ->
+      x = y.
+  Proof.
+    unfold unroll_between.
+    intros.
+    repeat break_if;
+      try find_eapply_lem_hyp between_bool_yz_antisymmetric;
+      congruence.
+  Qed.
+
+  Lemma unrolling_transitive :
+    forall h x y z,
+      unroll_between h x y = true ->
+      unroll_between h y z = true ->
+      unroll_between h x z = true.
+  Proof.
+    unfold unroll_between, between_bool.
+    intros.
+    repeat break_if; try subst; try congruence;
+    unfold bv_ltb in *;
+    rewrite Z.ltb_lt, Z.ltb_nlt in *;
+    omega.
+  Qed.
+
+  Lemma neq_in_id_implies_neq_in_z :
+    forall x y : id,
+      x <> y ->
+      z_of_id x <> z_of_id y.
+  Proof.
+    intros.
+    intro.
+    find_apply_lem_hyp (f_equal id_of_z).
+    repeat rewrite z_of_id_inv in *.
+    congruence.
+  Qed.
+
+  Lemma unrolling_total :
+    forall h x y,
+      unroll_between h x y = true \/
+      unroll_between h y x = true.
+  Proof.
+    unfold unroll_between, between_bool.
+    intros.
+    repeat break_if; try subst; try congruence; auto;
+      unfold bv_ltb in *;
+      try rewrite Z.ltb_lt, Z.ltb_nlt in *;
+      find_apply_lem_hyp neq_in_id_implies_neq_in_z;
+      try omega.
+      rewrite Z.ltb_nlt in *.
+      find_apply_lem_hyp neq_in_id_implies_neq_in_z;
+      try omega.
+  Qed.
+
+  Lemma unrolling_reflexive :
+    forall h x,
+      unroll_between h x x = true.
+  Proof.
+    unfold unroll_between, between_bool.
+    intros.
+    repeat break_if; try omega || subst; auto; try congruence.
+  Qed.
+
+  Definition unroll_between_ptr (h : name) (a b : pointer) :=
+    unroll_between (hash h) (ptrId a) (ptrId b).
+
+End IdentifierSpaces.
